catalyst-style encoding works

catalyst.fst
@@ -31,11 +31,6 @@ let rec dotp_is_correct #a x l y z =
   | hd :: tl ->
     dotp_is_correct x tl y z
 
-val cartp: #a:eqtype -> list a -> list a -> S.set (a&a)
-let rec cartp #a l1 l2 = match l1 with
-  | [] -> S.empty #(a&a)
-  | x::xs -> S.union (dotp x l2) (cartp xs l2)
-
 val cartp_prop: #a:eqtype -> list a -> list a -> S.set (a&a) -> prop
 let cartp_prop #a l1 l2 s = 
     forall x y. S.mem (x,y) s <==> S.mem x (mem l1) /\ S.mem y (mem l2)  
@@ -43,15 +38,67 @@ let cartp_prop #a l1 l2 s =
 #push-options "--query_stats --split_queries always"
 #set-options "--z3rlimit 1000"
 
-val cartp_is_correct:  #a:eqtype -> l1:list a -> l2:list a
-  -> Lemma (cartp_prop l1 l2 (cartp l1 l2))
-let rec cartp_is_correct l1 l2 = match l1 with
-  | [] -> ()
-  | x::xs -> cartp_is_correct xs l2
+val cartp: #a:eqtype -> l1:list a -> l2:list a -> 
+      s:S.set (a&a){cartp_prop l1 l2 s}
+let rec cartp #a l1 l2 = match l1 with
+  | [] -> S.empty #(a&a)
+  | x::xs -> S.union (dotp x l2) (cartp xs l2)
 
-
-val ord : #a:eqtype -> list a -> S.set (a & a)
-let rec ord #a l = match l with
+val ob_ord : #a:eqtype -> list a -> S.set (a & a)
+let rec ob_ord #a l = match l with
   | [] -> S.empty
-  | x::xs -> S.union (dotp x xs) (ord xs)
+  | x::xs -> S.union (dotp x xs) (ob_ord xs)
 
+val oa_ord : #a:eqtype -> list a -> S.set (a & a)
+let rec oa_ord #a l = match l with
+  | [] -> S.empty
+  | x::xs -> S.union (cartp xs [x]) (oa_ord xs)
+
+(*
+ * When using the provided set equality: `==`
+ * If you change `S.union (mem xs) (S.singleton x)` to 
+ * `S.union (S.singleton x) (mem xs)`, type checking would 
+ * fail because commutativity of set union w.r.t `==` is 
+ * never asserted.
+ * Using `=.` defined above fixes this problem as it is 
+ * defined in terms of `S.mem`, which is related to set 
+ * operations through a variety of lemmas.
+ *)
+val cons: #a:eqtype -> x:a -> xs:list a 
+  -> l:list a{mem l =. S.union (S.singleton x) (mem xs)
+          /\ ob_ord l =. S.union (dotp x xs) (ob_ord xs)
+          /\ oa_ord l =. S.union (cartp xs [x]) (oa_ord xs)}
+let cons x xs = x::xs
+
+let append_prop l1 l2 l = 
+  (mem l =. S.union (mem l1) (mem l2)) /\
+  (ob_ord l =. S.union (S.union (ob_ord l1) (ob_ord l2)) (cartp l1 l2)) /\
+  (oa_ord l =. S.union (S.union (oa_ord l1) (oa_ord l2)) (cartp l2 l1))
+
+val append: #a:eqtype -> l1:list a -> l2:list a 
+        -> l:list a{append_prop l1 l2 l}
+let rec append l1 l2 = match l1 with
+  | [] -> l2
+  | x::xs -> x::(append xs l2)
+
+val rev: #a:eqtype -> l1:list a 
+        -> l:list a{mem l =. mem l1 
+              /\ ob_ord l =. oa_ord l1 
+              /\ oa_ord l =. ob_ord l1} 
+let rec rev l1 = match l1 with
+  | [] -> []
+  | x::xs -> append (rev xs) [x]
+
+val filter_prop:#a:eqtype -> list a -> (a->bool) -> list a -> prop
+let filter_prop #a l1 f l =
+      (forall x. S.mem x (mem l) <==> S.mem x (mem l1) /\ f x)
+  /\  (forall x y. S.mem (x,y) (ob_ord l) 
+          <==> S.mem (x,y) (ob_ord l1) /\ f x /\ f y) 
+
+val filter: #a:eqtype -> f:(a -> bool) -> l1:list a
+      -> l:list a{filter_prop l1 f l}
+let rec filter #a f l1 = match l1 with
+  | [] -> []
+  | x::xs -> if f x then x::(filter f xs) else (filter f xs)
+
+  
